

find series soln of differential Eqn

$$(x-x^2)\frac{d^2y}{dx^2} + (1-5x)\frac{dy}{dx} - 4y = 0$$

$$P_0 = (x-x^2) \quad P_1 = (1-5x) \quad P_2 = -4$$

$$\text{at } x=0$$

$$P_0 = 0$$

$x=0$ is called

singular point

$$y = \sum_{k=0}^{\infty} a_k x^{m+k} \quad (1)$$

$$\frac{dy}{dx} = \sum_{k=0}^{\infty} a_k (m+k) x^{m+k-1} \quad (2)$$

$$\frac{d^2y}{dx^2} = \sum_{k=0}^{\infty} a_k (m+k)(m+k-1) x^{m+k-2} \quad (3)$$

Put $y, \frac{dy}{dx}, \frac{d^2y}{dx^2}$ from (1), (2), (3) in (A)

$$(x-x^2) \sum_{k=0}^{\infty} a_k (m+k)(m+k-1) x^{m+k-2} + (1-5x) \sum_{k=0}^{\infty} a_k (m+k) x^{m+k-1} - 4 \sum_{k=0}^{\infty} a_k x^{m+k} = 0$$

$$- 4 \sum_{k=0}^{\infty} a_k x^{m+k} = 0$$

$$\sum_{k=0}^{\infty} a_k (m+k)(m+k-1) x^{m+k-1} - \sum_{k=0}^{\infty} a_k (m+k)(m+k-1) x^{m+k} = 0$$

$$+ \sum_{k=0}^{\infty} a_k (m+k) x^{m+k-1} - 5 \sum_{k=0}^{\infty} a_k (m+k) x^{m+k} - 4 \sum_{k=0}^{\infty} a_k x^{m+k} = 0$$

$$\sum_{k=0}^{\infty} a_k \{ (m+k)(m+k-1) + (m+k) \} x^{m+k-1} - \sum_{k=0}^{\infty} a_k \{ (m+k) \}$$

$$(m+k-1) + 5(m+k) + 4 \} x^{m+k} = 0$$

$$\sum_{k=0}^{\infty} a_k \{ (m+k)^2 - (m+k) + (m+k) \} x^{m+k-1} = \sum_{k=0}^{\infty} a_k$$

$$\{ (m+k)^2 - (m+k) + 5(m+k) + 4 \} x^{m+k} = 0$$

$$\sum_{k=0}^{\infty} a_k \{(m+k)^2 x^{m+k-1} - \sum_{k=0}^{\infty} a_k \{(m+k)^2 + 4(m+k) + 4\} x^{m+k} = 0$$

on equating lowest degree term i.e. x^{m-1} which is obtained by putting $k=0$ in $I^{st} \Sigma$ only

$$a_0 m^2 = 0 \text{ but } a_0 \neq 0 \Rightarrow m = 0, 0$$

on Equating coefficient of x^m which is obtained by putting $k=1$ in $I^{st} \Sigma$ and $k=0$ in $II^{nd} \Sigma$

$$\Rightarrow a_1(m+1)^2 - a_0 \{m^2 + 4m + 4\} = 0$$

$$a_1 = \frac{a_0(m+2)^2}{(m+1)^2}$$

on Equating coefficient of x^{m+1} which is obtained by putting $k=2$ in $I^{st} \Sigma$ and $k=1$ in $II^{nd} \Sigma$

$$a_2(m+2)^2 - a_1 \{(m+1)^2 + 4(m+1) + 4\} = 0$$

$$a_2 = \frac{a_1 \{(m+1)^2 + 4(m+1) + 4\}}{(m+2)^2}$$

$$a_2 = \frac{\{(m+1)^2 + 4(m+1) + 4\} a_0(m+2)^2}{(m+2)^2 (m+1)^2}$$

$$a_2 = (4m+8)a_0$$

on Equating coefficient of x^{m+2} which is obtained by putting $k=3$ in $I^{st} \Sigma$ and $k=2$ in $II^{nd} \Sigma$

$$a_3(m+3)^2 - a_2 \{(m+2)^2 + 4(m+2) + 4\} = 0$$

$$a_3 = \frac{a_2 \{(m+2)^2 + 4(m+2) + 4\}}{(m+3)^2}$$

$$a_3 = \frac{\{(m+2)^2 + 4(m+2) + 4\} (4m+8) a_0}{(m+3)^2}$$

Put a_0, a_1, a_2, a_3 in -----

$$\text{In } y = \sum_{k=0}^{\infty} a_k x^{m+k} \quad \text{--- (1)}$$

$$y = a_0 x^m + a_1 x^{m+1} + a_2 x^{m+2} + a_3 x^{m+3} + \dots$$

$$y = a_0 x^m \left\{ a_0 + \frac{a_0 (m+2)^2}{(m+1)^2} x + \{(4m+8) a_0\} x^2 \right.$$

$$\left. + \frac{\{(m+2)^2 + 4(m+2) + 4\} \{4m+8\} a_0}{(m+3)^2} x^3 \right\}$$

Ans